CartesianClosed.v
@@ -2,7 +2,7 @@ Add Rec LoadPath "/home/zeimer/Code/Coq".
 
 Require Export Cat.
 Require Import InitTerm.
-Require Import BinProdCoprod.
+Require Import Cat.BinProdCoprod.
 Require Import Exponential.
 
 Class cartesian_closed (C : Cat) : Type :=
@@ -12,21 +12,15 @@ Class cartesian_closed (C : Cat) : Type :=
     ccc_exp :> has_exponentials C
 }.
 
-Arguments term [C] [has_term].
-Arguments delete [C] [has_term] _.
-Arguments diag [C] [has_products] _ _ _ _ _.
-
-Theorem id_unique_left' : forall (C : Cat) (X Y : Ob C)
-    (f : Hom X Y) (g : Hom Y X), f .> g .> f == f -> f .> g == id X.
-Proof.
-  intros. apply id_unique_left. intros.
-Abort.
+Coercion ccc_term : cartesian_closed >-> has_term.
+Coercion ccc_prod : cartesian_closed >-> has_products.
+Coercion ccc_exp : cartesian_closed >-> has_exponentials.
 
 Theorem prod_term_iso : forall (C : Cat) (X : Ob C)
     (ht : has_term C) (hp : has_products C),
-        prodOb term X ~ X.
+        prodOb (term C) X ~ X.
 Proof.
-  symmetry. (*destruct ht, hp*) intros; red; simpl.
+  (*symmetry. (*destruct ht, hp*) intros; red; simpl.
   pose (f := diag term X X (delete X) (id X)).
   exists f; red. exists (proj2 term X). unfold f.
   destruct (is_product term X X (delete X) (id X)) as [[H1 H2] H3].
@@ -41,7 +35,7 @@ Check id_unique_left. apply id_unique_left. intros.
     destruct (is_product term X (prodOb term X) (delete _) (proj2 term X)).
       destruct H0. specialize (H4 (id _)). cat.
       assert (delete (prodOb term X) == proj1 term X).
-      destruct ht. simpl in *. rewrite <- is_terminal. reflexivity.
+      destruct ht. simpl in *. rewrite <- is_terminal. reflexivity.*)
 Abort. (*
       destruct (is_terminal (prodOb term X) (proj1 term X)).
 
@@ -50,3 +44,32 @@ Abort. (*
     rewrite <- ProductFunctor_fmap_pres_id.
       unfold ProductFunctor_fmap.
       *)
+
+Theorem exp_term_dom :
+    forall (C : Cat) (ccc : cartesian_closed C) (Y : Ob C),
+    expOb (term C) Y ~ Y.
+Proof.
+  symmetry; red.
+  exists (curry proj1). red.
+  exists (diag (id (expOb (term C) Y)) (delete _) .> eval).
+  destruct ccc, ccc_term0, ccc_prod0, ccc_exp0; simpl in *.
+  do 2 red in is_exponential; simpl in *.
+  split.
+Abort.
+
+Theorem exp_term_cod :
+    forall (C : Cat) (ccc : cartesian_closed C) (Y : Ob C),
+    expOb Y (term C) ~ term C.
+Proof.
+  red; intros.
+  exists (delete _). red. exists (curry proj1).
+  split.
+    Focus 2. destruct ccc, ccc_term0; simpl in *.
+      rewrite is_terminal. rewrite <- (is_terminal _ (id term)).
+        reflexivity.
+    destruct ccc, ccc_term0; simpl in *.
+    destruct ccc_exp0; do 2 red in is_exponential; simpl in *.
+    destruct (is_exponential Y term (expOb Y term) (eval _ _)).
+      specialize (H0 (id (expOb Y term))).
+      rewrite <- H0.
+Abort.
