Instances/Set/CoqSet.v
@@ -305,26 +305,11 @@ Proof.
   unfold coequalizer; simpl; intros. cat. f_equal.
 *)
 
-(* TODO: Hom functor here *)
-
 Instance CoqSet_has_exponentials : has_exponentials CoqSet :=
 {
     expOb := fun X Y : Set => X -> Y;
-    eval := fun (X Y : Set) (fx : prodOb (X -> Y) X) => (fst fx) (snd fx)
-}.
-Proof.
-  red; simpl; intros. exists (fun (z : Z) (x : X) => e (z, x)).
-  red; split.
-    destruct x. simpl. reflexivity.
-    simpl. intros f H z. extensionality x.
-      rewrite <- H. simpl. reflexivity.
-Defined.
-
-Instance CoqSet_has_exponentials' : has_exponentials' CoqSet :=
-{
-    expOb' := fun X Y : Set => X -> Y;
-    eval' := fun (X Y : Set) (fx : prodOb (X -> Y) X) => (fst fx) (snd fx);
-    curry' := fun (X Y Z : Set) (f : Z * X -> Y) (z : Z) =>
+    eval := fun (X Y : Set) (fx : prodOb (X -> Y) X) => (fst fx) (snd fx);
+    curry := fun (X Y Z : Set) (f : Z * X -> Y) (z : Z) =>
       fun x : X => f (z, x)
 }.
 Proof.
