README.md
@@ -19,9 +19,7 @@ Fix:
  * Prove that dual is involution with respect to equality and then remove the axiom I'm currently using.
  * Write new unique ismorphicness theorems for products (the isos have to be compatible with the projections).
  * Check whether big\_product is properly defined (there was an error in big\_product\_skolem).
- * Give some structure to the modules, e.g. Sgr should be called Instances.Set.Sgr. Solution: each subdirectory has to have its own makefile...
  * Maybe I should use Proper more? Looks like having "Proper ..." in context makes rewriting easy. Maybe there should be separate Proper instances for each variable, like x == x' -> R x y -> R x' y?
- * Make sure everything works with the new makefile.
 
 General:
  * Implement a tactic to decide equality of morphisms based on a tactic that decides whether two elements of a monoid are equal (was it described in Coq'Art?). This will be very hard, but fruitful.
@@ -36,7 +34,6 @@ Instances:
  * Find a general boilerplate for a file with concrete category — apply it to all instances.
  * Define heterogenous apartoids.
  * Implement prosets and semigroups wth respect to setoids/apartoids etc.
- * Implement some examples of functors (like the Hom functor).
 
 Further ideas:
  * Implement concrete categories and use them for theorems about individual categories.
